Metatheory/TRS/FirstOrder/Rules.lean
@@ -20,6 +20,10 @@ structure Rule (sig : Signature) where
   lhs : Term sig
   rhs : Term sig
 
+noncomputable instance instDecidableEqRule {sig : Signature} : DecidableEq (Rule sig) := by
+  classical
+  exact Classical.decEq _
+
 /-- A set of rewrite rules. -/
 abbrev RuleSet (sig : Signature) := Rule sig -> Prop
 
